theories/base.v
@@ -10,10 +10,3 @@ Global Set Default Proof Using "Type".
 Global Unset Program Cases.
 Global Set Keyed Unification.
 Global Set Default Goal Selector "!".
-
-Lemma TraceStep' {EV} κs κs' (m : module EV) σ2 σ1 σ3 κ :
-  m.(m_step) σ1 κ σ2 →
-  κs = option_list (Vis <$> κ) ++ κs' →
-  σ2 ~{ m, κs' }~> σ3 →
-  σ1 ~{ m, κs }~> σ3.
-Proof. move => ? -> ?. by apply: TraceStep. Qed.
